iris_heap_lang/primitive_laws.v
@@ -75,7 +75,7 @@ Qed.
 
 (** Since we use an [option val] instance of [gen_heap], we need to overwrite
 the notations.  That also helps for scopes and coercions. *)
-Notation "l ↦ dq v" := (mapsto (L:=loc) (V:=option val) l dq (Some v%V))
+Notation "l ↦ dq v" := (pointsto (L:=loc) (V:=option val) l dq (Some v%V))
   (at level 20, dq custom dfrac at level 1, format "l  ↦ dq  v") : bi_scope.
 
 (** Same for [gen_inv_heap], except that these are higher-order notations so to
@@ -83,19 +83,19 @@ make setoid rewriting in the predicate [I] work we need actual definitions
 here. *)
 Section definitions.
   Context `{!heapGS_gen hlc Σ}.
-  Definition inv_mapsto_own (l : loc) (v : val) (I : val → Prop) : iProp Σ :=
-    inv_mapsto_own l (Some v) (from_option I False).
-  Definition inv_mapsto (l : loc) (I : val → Prop) : iProp Σ :=
-    inv_mapsto l (from_option I False).
+  Definition inv_pointsto_own (l : loc) (v : val) (I : val → Prop) : iProp Σ :=
+    inv_pointsto_own l (Some v) (from_option I False).
+  Definition inv_pointsto (l : loc) (I : val → Prop) : iProp Σ :=
+    inv_pointsto l (from_option I False).
 End definitions.
 
-Global Instance: Params (@inv_mapsto_own) 4 := {}.
-Global Instance: Params (@inv_mapsto) 3 := {}.
+Global Instance: Params (@inv_pointsto_own) 4 := {}.
+Global Instance: Params (@inv_pointsto) 3 := {}.
 
 Notation inv_heap_inv := (inv_heap_inv loc (option val)).
-Notation "l '↦_' I □" := (inv_mapsto l I%stdpp%type)
+Notation "l '↦_' I □" := (inv_pointsto l I%stdpp%type)
   (at level 20, I at level 9, format "l  '↦_' I  '□'") : bi_scope.
-Notation "l ↦_ I v" := (inv_mapsto_own l v I%stdpp%type)
+Notation "l ↦_ I v" := (inv_pointsto_own l v I%stdpp%type)
   (at level 20, I at level 9, format "l  ↦_ I  v") : bi_scope.
 
 Section lifting.
@@ -202,15 +202,15 @@ Qed.
 (** We need to adjust the [gen_heap] and [gen_inv_heap] lemmas because of our
 value type being [option val]. *)
 
-Lemma mapsto_valid l dq v : l ↦{dq} v -∗ ⌜✓ dq⌝.
-Proof. apply mapsto_valid. Qed.
-Lemma mapsto_valid_2 l dq1 dq2 v1 v2 :
+Lemma pointsto_valid l dq v : l ↦{dq} v -∗ ⌜✓ dq⌝.
+Proof. apply pointsto_valid. Qed.
+Lemma pointsto_valid_2 l dq1 dq2 v1 v2 :
   l ↦{dq1} v1 -∗ l ↦{dq2} v2 -∗ ⌜✓ (dq1 ⋅ dq2) ∧ v1 = v2⌝.
 Proof. iIntros "H1 H2". iCombine "H1 H2" gives %[? [= ?]]. done. Qed.
-Lemma mapsto_agree l dq1 dq2 v1 v2 : l ↦{dq1} v1 -∗ l ↦{dq2} v2 -∗ ⌜v1 = v2⌝.
+Lemma pointsto_agree l dq1 dq2 v1 v2 : l ↦{dq1} v1 -∗ l ↦{dq2} v2 -∗ ⌜v1 = v2⌝.
 Proof. iIntros "H1 H2". iCombine "H1 H2" gives %[_ [= ?]]. done. Qed.
 
-Global Instance mapsto_combine_sep_gives l dq1 dq2 v1 v2 : 
+Global Instance pointsto_combine_sep_gives l dq1 dq2 v1 v2 : 
   CombineSepGives (l ↦{dq1} v1) (l ↦{dq2} v2) ⌜✓ (dq1 ⋅ dq2) ∧ v1 = v2⌝ | 20. 
   (* We provide an instance with lower cost than the gen_heap instance
      to avoid having to deal with Some v1 = Some v2 *)
@@ -219,71 +219,71 @@ Proof.
   iCombine "H1 H2" gives %[? [=->]]. eauto.
 Qed.
 
-Lemma mapsto_combine l dq1 dq2 v1 v2 :
+Lemma pointsto_combine l dq1 dq2 v1 v2 :
   l ↦{dq1} v1 -∗ l ↦{dq2} v2 -∗ l ↦{dq1 ⋅ dq2} v1 ∗ ⌜v1 = v2⌝.
 Proof.
   iIntros "Hl1 Hl2". by iCombine "Hl1 Hl2" as "$" gives %[_ ->].
 Qed.
 
-Lemma mapsto_frac_ne l1 l2 dq1 dq2 v1 v2 :
+Lemma pointsto_frac_ne l1 l2 dq1 dq2 v1 v2 :
   ¬ ✓(dq1 ⋅ dq2) → l1 ↦{dq1} v1 -∗ l2 ↦{dq2} v2 -∗ ⌜l1 ≠ l2⌝.
-Proof. apply mapsto_frac_ne. Qed.
-Lemma mapsto_ne l1 l2 dq2 v1 v2 : l1 ↦ v1 -∗ l2 ↦{dq2} v2 -∗ ⌜l1 ≠ l2⌝.
-Proof. apply mapsto_ne. Qed.
+Proof. apply pointsto_frac_ne. Qed.
+Lemma pointsto_ne l1 l2 dq2 v1 v2 : l1 ↦ v1 -∗ l2 ↦{dq2} v2 -∗ ⌜l1 ≠ l2⌝.
+Proof. apply pointsto_ne. Qed.
 
-Lemma mapsto_persist l dq v : l ↦{dq} v ==∗ l ↦□ v.
-Proof. apply mapsto_persist. Qed.
+Lemma pointsto_persist l dq v : l ↦{dq} v ==∗ l ↦□ v.
+Proof. apply pointsto_persist. Qed.
 
-Global Instance inv_mapsto_own_proper l v :
-  Proper (pointwise_relation _ iff ==> (≡)) (inv_mapsto_own l v).
+Global Instance inv_pointsto_own_proper l v :
+  Proper (pointwise_relation _ iff ==> (≡)) (inv_pointsto_own l v).
 Proof.
-  intros I1 I2 HI. rewrite /inv_mapsto_own. f_equiv=>-[w|]; last done.
+  intros I1 I2 HI. rewrite /inv_pointsto_own. f_equiv=>-[w|]; last done.
   simpl. apply HI.
 Qed.
-Global Instance inv_mapsto_proper l :
-  Proper (pointwise_relation _ iff ==> (≡)) (inv_mapsto l).
+Global Instance inv_pointsto_proper l :
+  Proper (pointwise_relation _ iff ==> (≡)) (inv_pointsto l).
 Proof.
-  intros I1 I2 HI. rewrite /inv_mapsto. f_equiv=>-[w|]; last done.
+  intros I1 I2 HI. rewrite /inv_pointsto. f_equiv=>-[w|]; last done.
   simpl. apply HI.
 Qed.
 
-Lemma make_inv_mapsto l v (I : val → Prop) E :
+Lemma make_inv_pointsto l v (I : val → Prop) E :
   ↑inv_heapN ⊆ E →
   I v →
   inv_heap_inv -∗ l ↦ v ={E}=∗ l ↦_I v.
-Proof. iIntros (??) "#HI Hl". iApply make_inv_mapsto; done. Qed.
-Lemma inv_mapsto_own_inv l v I : l ↦_I v -∗ l ↦_I □.
-Proof. apply inv_mapsto_own_inv. Qed.
+Proof. iIntros (??) "#HI Hl". iApply make_inv_pointsto; done. Qed.
+Lemma inv_pointsto_own_inv l v I : l ↦_I v -∗ l ↦_I □.
+Proof. apply inv_pointsto_own_inv. Qed.
 
-Lemma inv_mapsto_own_acc_strong E :
+Lemma inv_pointsto_own_acc_strong E :
   ↑inv_heapN ⊆ E →
   inv_heap_inv ={E, E ∖ ↑inv_heapN}=∗ ∀ l v I, l ↦_I v -∗
     (⌜I v⌝ ∗ l ↦ v ∗ (∀ w, ⌜I w ⌝ -∗ l ↦ w ==∗
-      inv_mapsto_own l w I ∗ |={E ∖ ↑inv_heapN, E}=> True)).
+      inv_pointsto_own l w I ∗ |={E ∖ ↑inv_heapN, E}=> True)).
 Proof.
   iIntros (?) "#Hinv".
-  iMod (inv_mapsto_own_acc_strong with "Hinv") as "Hacc"; first done.
+  iMod (inv_pointsto_own_acc_strong with "Hinv") as "Hacc"; first done.
   iIntros "!>" (l v I) "Hl". iDestruct ("Hacc" with "Hl") as "(% & Hl & Hclose)".
   iFrame "%∗". iIntros (w) "% Hl". iApply "Hclose"; done.
 Qed.
 
-Lemma inv_mapsto_own_acc E l v I:
+Lemma inv_pointsto_own_acc E l v I:
   ↑inv_heapN ⊆ E →
   inv_heap_inv -∗ l ↦_I v ={E, E ∖ ↑inv_heapN}=∗
     (⌜I v⌝ ∗ l ↦ v ∗ (∀ w, ⌜I w ⌝ -∗ l ↦ w ={E ∖ ↑inv_heapN, E}=∗ l ↦_I w)).
 Proof.
   iIntros (?) "#Hinv Hl".
-  iMod (inv_mapsto_own_acc with "Hinv Hl") as "(% & Hl & Hclose)"; first done.
+  iMod (inv_pointsto_own_acc with "Hinv Hl") as "(% & Hl & Hclose)"; first done.
   iFrame "%∗". iIntros "!>" (w) "% Hl". iApply "Hclose"; done.
 Qed.
 
-Lemma inv_mapsto_acc l I E :
+Lemma inv_pointsto_acc l I E :
   ↑inv_heapN ⊆ E →
   inv_heap_inv -∗ l ↦_I □ ={E, E ∖ ↑inv_heapN}=∗
     ∃ v, ⌜I v⌝ ∗ l ↦ v ∗ (l ↦ v ={E ∖ ↑inv_heapN, E}=∗ ⌜True⌝).
 Proof.
   iIntros (?) "#Hinv Hl".
-  iMod (inv_mapsto_acc with "Hinv Hl") as ([v|]) "(% & Hl & Hclose)"; [done| |done].
+  iMod (inv_pointsto_acc with "Hinv Hl") as ([v|]) "(% & Hl & Hclose)"; [done| |done].
   iIntros "!>". iExists (v). iFrame "%∗".
 Qed.
 
@@ -305,8 +305,8 @@ Proof.
   rewrite big_opM_singleton; iDestruct "Hvs" as "[$ Hvs]". by iApply "IH".
 Qed.
 
-Lemma heap_array_to_seq_mapsto l v (n : nat) :
-  ([∗ map] l' ↦ ov ∈ heap_array l (replicate n v), gen_heap.mapsto l' (DfracOwn 1) ov) -∗
+Lemma heap_array_to_seq_pointsto l v (n : nat) :
+  ([∗ map] l' ↦ ov ∈ heap_array l (replicate n v), gen_heap.pointsto l' (DfracOwn 1) ov) -∗
   [∗ list] i ∈ seq 0 n, (l +ₗ (i : nat)) ↦ v.
 Proof.
   iIntros "Hvs". iInduction n as [|n] "IH" forall (l); simpl.
@@ -337,7 +337,7 @@ Proof.
   iMod (steps_auth_update_S with "Hsteps") as "Hsteps".
   iModIntro; do 2 (iSplit; first done). iFrame "Hσ Hκs Hsteps". iApply "HΦ".
   iApply big_sepL_sep. iSplitL "Hl".
-  - by iApply heap_array_to_seq_mapsto.
+  - by iApply heap_array_to_seq_pointsto.
   - iApply (heap_array_to_seq_meta with "Hm"). by rewrite replicate_length.
 Qed.
 Lemma wp_allocN_seq s E v n :
